save

extraction/chord/ml/ChordShedArrangement.ml
@@ -1,0 +1,100 @@
+open Printf
+open String
+
+open ExtractedChordShed
+
+let show_pointer p =
+  string_of_int (id_of p)
+
+let show_addr_list l =
+  sprintf "[%s]" (String.concat "; " (map (sprintf "%d") l))
+
+let show_pointer_list ps =
+  let strs = map show_pointer ps in
+  "[" ^ String.concat ", " strs ^ "]"
+
+let map_default f d = function
+  | None -> d
+  | Some v -> f v
+
+let show_opt_pointer p =
+  map_default show_pointer "None" p
+
+let show_payload = function
+  | GetBestPredecessor p -> "GetBestPredecessor " ^ show_pointer p
+  | GotBestPredecessor p -> "GotBestPredecessor " ^ show_pointer p
+  | GetSuccList -> "GetSuccList"
+  | GotSuccList ps -> "GotSuccList " ^ show_pointer_list ps
+  | GetPredAndSuccs -> "GetPredAndSuccs"
+  | GotPredAndSuccs (pred, succs) -> "GotPredAndSuccs " ^ show_opt_pointer pred ^ " " ^ show_pointer_list succs
+  | Notify -> "Notify"
+  | Ping -> "Ping"
+  | Pong -> "Pong"
+  | Busy -> "Busy"
+
+let show_timeout = function
+  | Tick -> "Tick"
+  | KeepaliveTick -> "KeepaliveTick"
+  | Request (a, p) -> sprintf "Request %d %s" a (show_payload p)
+
+(* just deliver a message *)
+let next gst n =
+  let n' = n mod (List.length (msgs gst)) in
+  Op_deliver (n', (List.nth (msgs gst) n'))
+
+let init_nodes =
+    [10;30;50;70;90]
+let pred_for_init = function
+  | 10 -> 90
+  | 30 -> 10
+  | 50 -> 30
+  | 70 -> 50
+  | 90 -> 70
+  | _ -> 0
+
+let succs_for_init = function
+  | 10 -> [30;50]
+  | 30 -> [50;70]
+  | 50 -> [70;90]
+  | 70 -> [90;10]
+  | 90 -> [10;30]
+  | _ -> []
+let mp = make_pointer (fun a -> a mod 256)
+let init_sigma h =
+    if List.mem h init_nodes
+    then Some ({ ptr = mp h
+              ; pred = Some (mp (pred_for_init h))
+              ; succ_list = map mp (succs_for_init h)
+              ; known = mp 10
+              ; joined = true
+              ; rectify_with = None
+              ; cur_request = None
+              ; delayed_queries = [] })
+    else None
+
+let init =
+    { nodes = init_nodes
+    ; failed_nodes = []
+    ; timeouts = (fun _ -> [])
+    ; sigma = init_sigma
+    ; msgs = []
+    ; trace = [] }
+
+module ChordArrangement = struct
+  type net = (addr, payload, data, timeout) global_state
+  type operation = (addr, payload, timeout) ExtractedChordShed.operation
+  let run = run 
+  let next = next
+  let inits = [("hardcoded", init)]
+  let netpreds = [all_nodes_live_netpred, np_const_true]
+  let show_operation = function
+  | Op_start (a, ks) -> 
+      sprintf "op_start %d %s" a (show_addr_list ks)
+  | Op_fail a -> 
+      sprintf "op_fail %d" a
+  | Op_timeout (a, t) ->
+      sprintf "op_timeout %d %s" a (show_timeout t)
+  | Op_deliver (n, (src, (dst, p))) ->
+      sprintf "op_deliver %d %d %d %s" n src dst (show_payload p)
+  let show_net gst = "there should be a network here."
+end
