extraction/lib/ShedShim.ml
@@ -1,0 +1,87 @@
+open ExtractedShed
+open List
+open Random
+
+module type SHED_ARRANGEMENT = sig
+    type net
+    type operation
+    val run : net -> operation -> net option
+    val next : net -> nat -> operation
+    (* assoc list from identifiers to starting states *)
+    val inits : (string * net) list
+    val netpreds : (net netpred) list
+    val tracepreds : ((net, operation) tracepred) list
+    val show_operation : operation -> string
+    val show_net : net -> string
+end
+
+let implode l =
+  let res = String.create (length l) in
+  let rec imp i = function
+    | [] ->
+       res
+    | c :: l ->
+       res.[i] <- c;
+       imp (i + 1) l in
+  imp 0 l
+
+module Shim (A: SHED_ARRANGEMENT) = struct
+    type cfg =
+        { netpreds : (A.net netpred) list
+        ; tracepreds : ((A.net, A.operation) tracepred) list
+        ; init : A.net
+        ; depth : int }
+
+    let print_occ occ =
+      print_endline (A.show_operation occ.occ_op)
+
+    let print_np_res i (np, l) = 
+      print_endline ((implode np.np_name) ^ ": " ^ string_of_bool (nth l i))
+
+    let show_tp_result = function
+      | Tp_True -> "tp_True"
+      | Tp_False -> "tp_False"
+      | Tp_Maybe -> "tp_Maybe"
+      
+    let print_tp_res i (tp, l) =
+      print_endline ((implode tp.tp_name) ^ ": " ^ show_tp_result (nth l i))
+
+    let print_step res i occ =
+      print_occ occ;
+      iter (print_np_res i) (ts_netpreds A.run res);
+      iter (print_tp_res i) (ts_tracepreds A.run res)
+
+    let print_res res =
+      iteri (print_step res) res.ts_trace;
+      print_endline "";
+      print_endline (A.show_net res.ts_latest)
+                      
+    let find_np_by_name s =
+      find (fun np -> s = np.np_name) A.netpreds
+             
+    let find_tp_by_name s =
+      find (fun tp -> s = tp.tp_name) A.tracepreds
+
+    let run_test cfg =
+      let res = random_test A.run cfg.netpreds cfg.tracepreds cfg.init A.next cfg.depth in
+      print_res res
+                  
+    let main = 
+      let nps = ref [] in
+      let tps = ref [] in
+      let n = ref 5 in
+      let init = ref "" in
+      let add_np s = nps := find_np_by_name s :: !nps in
+      let add_tp s = tps := find_tp_by_name s :: !tps in
+      let opts =
+          [ ("-np", Arg.String add_np, "network predicate to check")
+          ; ("-tp", Arg.String add_tp, "network predicate to check")
+          ; ("-depth", Arg.Set_int n, "number of steps to take")
+          ; ("-init", Arg.Set_string init, "name of initial state") ] in
+      Arg.parse opts (fun _ -> ());
+      run_test { netpreds = !nps
+               ; tracepreds = !tps
+               ; init = assoc !init A.inits 
+               ; depth = !n }
+end
+
