extraction/chord/coq/ExtractChord.v
@@ -4,6 +4,8 @@ Require Import ExtrOcamlNatInt.
 Require Import ExtrOcamlString.
 
 Require Import Chord.
+Require Import ChordShed.
+Require Import Shed.
 
 Definition SUCC_LIST_LEN := 2.
 
@@ -23,3 +25,5 @@ Definition handleTimeout : addr -> data -> timeout -> res :=
   timeout_handler hash.
 
 Extraction "extraction/chord/coq/ExtractedChord.ml" init handleNet handleTick handleTimeout is_request closes_request.
+
+Extraction "extraction/chord/coq/ExtractedChordShed.ml" chord_test all_nodes_live_netpred np_const_true tp_const_true.
