shed/ChordShed.v
@@ -1,0 +1,213 @@
+Require Import List.
+Require Import mathcomp.ssreflect.ssreflect.
+Require Import StructTact.StructTactics.
+Require Import StructTact.Before.
+
+Require Import Chord.
+Require Import ChordProof.
+Require Import DynamicNet.
+Require Import DynamicShed.
+Require Import Shed.
+
+Section ChordShed.
+
+  Set Bullet Behavior "Strict Subproofs".
+
+  Variable SUCC_LIST_LEN : nat.
+  Variable hash : addr -> id.
+
+  Notation global_state := (global_state addr payload data timeout).
+  Notation start_handler := (start_handler SUCC_LIST_LEN hash).
+  Notation recv_handler := (recv_handler SUCC_LIST_LEN hash).
+  Notation timeout_handler := (timeout_handler hash).
+  Notation step_dynamic := (step_dynamic addr addr_eq_dec payload data timeout timeout_eq_dec start_handler recv_handler timeout_handler timeout_constraint failure_constraint).
+  Notation operation := (operation addr payload timeout).
+  Notation msg_eq_dec := (msg_eq_dec addr addr_eq_dec payload payload_eq_dec).
+  Notation sigma := (sigma addr payload data timeout).
+  Notation nodes := (nodes addr payload data timeout).
+  Notation failed_nodes := (failed_nodes addr payload data timeout).
+
+  Definition request_response_pair_dec : forall p m,
+      {request_response_pair p m} + {~ request_response_pair p m}.
+  Proof.
+    intuition.
+    destruct p;
+      destruct m;
+      try now (auto using pair_GetBestPredecessor, pair_GetSuccList, pair_GetPredAndSuccs, pair_Ping) ||
+          (right; intro H_p; now inv H_p).
+  Qed.
+
+  Definition constraint_dec_helper :
+    forall (l : list (addr * (addr * payload))) dst h p,
+      (* parens here to avoid clashing w/ some ssreflect notation *)
+      {(forall m, request_response_pair p m -> ~ In (dst, (h, m)) l)} +
+      {~ (forall m, request_response_pair p m -> ~ In (dst, (h, m)) l)}.
+  Proof.
+    intros.
+    induction l.
+    - left.
+      easy.
+    - destruct IHl.
+      + destruct a as [from [to m]].
+        destruct (request_response_pair_dec p m);
+          destruct (addr_eq_dec dst from);
+          destruct (addr_eq_dec h to);
+          subst_max.
+        { right.
+          intro H_f.
+          apply H_f in r.
+          auto with datatypes. }
+        { left.
+          intuition.
+          find_apply_lem_hyp in_inv.
+          break_or_hyp.
+          -- repeat tuple_inversion.
+             auto.
+          -- eapply n; eauto. }
+        all: (left;
+               intuition;
+               find_apply_lem_hyp in_inv;
+               break_or_hyp;
+               try now (repeat tuple_inversion; auto);
+               eapply n; eauto).
+      + destruct a as [from [to m]].
+        destruct (request_response_pair_dec p m);
+          destruct (addr_eq_dec dst from);
+          destruct (addr_eq_dec h to);
+          subst_max.
+        { right.
+          intro H.
+          eapply H; eauto with datatypes. }
+        all: (right;
+               intro H;
+               apply n;
+               intros m0 H_pair H_in;
+               eapply H; eauto with datatypes).
+  Defined.
+
+  Definition timeout_constraint_dec : forall gst h t,
+      {timeout_constraint gst h t} + {~ timeout_constraint gst h t}.
+  Proof.
+    intros.
+    destruct t.
+    - left.
+      apply Tick_unconstrained.
+    - left.
+      apply KeepaliveTick_unconstrained.
+    - destruct (In_dec addr_eq_dec a (failed_nodes gst)).
+      * assert ({(forall m, request_response_pair p m -> ~ In (a, (h, m)) (msgs addr payload data timeout gst))} + {~ (forall m, request_response_pair p m -> ~ In (a, (h, m)) (msgs addr payload data timeout gst))}) by apply constraint_dec_helper.
+        destruct H.
+        + left.
+          eapply Request_needs_dst_dead_and_no_msgs; eauto.
+        + right.
+          intro H_t.
+          inv H_t.
+          easy.
+      * right.
+        intro H_t.
+        inv H_t.
+        easy.
+  Defined.
+
+  Definition live_succ_exists_dec :
+    forall gst l,
+      {  (exists s xs ys, live_node gst s /\ l = xs ++ s :: ys /\ (forall o, In o xs -> dead_node gst o))} +
+      {~ (exists s xs ys, live_node gst s /\ l = xs ++ s :: ys /\ (forall o, In o xs -> dead_node gst o))}.
+  Admitted.
+
+  Definition failure_constraint_helper :
+    forall gst h st,
+      sigma gst h = Some st ->
+      {(exists s, best_succ gst h s)} + {~ exists s, best_succ gst h s}.
+  Proof.
+    intros.
+    unfold best_succ.
+    set (addrs := map addr_of (succ_list st)).
+    destruct (live_succ_exists_dec gst addrs);
+      destruct (live_node_dec gst h).
+    - left.
+      break_exists_exists.
+      exists st.
+      break_exists_exists.
+      intuition.
+    - right.
+      move => H_bs.
+      break_exists.
+      break_and.
+      auto.
+    - right.
+      move => H_bs.
+      apply n.
+      break_exists_exists.
+      break_exists_name st'.
+      break_exists_exists.
+      intuition.
+      assert (st' = st).
+        by (find_rewrite; find_inversion).
+      subst.
+      easy.
+    - right.
+      move => H_bs.
+      break_exists.
+      break_and.
+      auto.
+  Defined.
+
+  Definition has_state (gst : global_state) (h : addr) : Prop :=
+    exists st, sigma gst h = Some st.
+
+  Definition has_state_dec :
+    forall gst h,
+      {has_state gst h} + {~has_state gst h}.
+  Proof.
+    intuition.
+    destruct (sigma gst h) as [st|] eqn:H_st.
+    - left.
+      now exists st.
+    - right.
+      move => H_hs.
+      destruct H_hs.
+      congruence.
+  Defined.
+
+  Definition failure_constraint_dec : forall gst,
+      {failure_constraint gst} + {~ failure_constraint gst}.
+  Proof.
+    unfold failure_constraint, live_node_in_succ_lists.
+    move => gst.
+    destruct (Forall_dec (live_node gst) (live_node_dec gst) (nodes gst)) as [H_st | H_st].
+    - rewrite -> Forall_forall in H_st.
+      assert (forall h, In h (nodes gst) -> {(exists s, best_succ gst h s)} + {~ exists s, best_succ gst h s}).
+      { move => h H_node.
+        set H_hl := H_st h H_node.
+        apply live_node_means_state_exists in H_hl.
+        destruct (sigma gst h) eqn:H_sig.
+        + eapply failure_constraint_helper.
+          repeat find_rewrite.
+          eauto.
+        + exfalso.
+          break_exists.
+          congruence. }
+  Admitted.
+
+  Definition all_nodes_live (gst : global_state) : Prop :=
+    Forall (live_node gst) (nodes gst).
+    
+  Definition all_nodes_live_dec :
+    forall gst,
+      {all_nodes_live gst} + {~ all_nodes_live gst}.
+  Proof.
+    move => gst.
+    apply Forall_dec.
+    exact: live_node_dec.
+  Qed.
+
+  Definition all_nodes_live_netpred : netpred global_state :=
+    {| np_prop := all_nodes_live;
+       np_dec := all_nodes_live_dec;
+       np_name := "all_nodes_live" |}.
+
+  Notation run := (run addr payload data timeout addr_eq_dec payload_eq_dec timeout_eq_dec start_handler recv_handler timeout_handler timeout_constraint timeout_constraint_dec).
+  Definition chord_test := random_test global_state operation run.
+
+End ChordShed.
