shed/Shed.v
@@ -1,0 +1,254 @@
+Require Import List.
+Import ListNotations.
+Require Import PeanoNat.
+Require Import String.
+Require Import ExtrOcamlString.
+Require Import ExtrOcamlBasic.
+
+Require Import Coqlib.
+Require Import InfSeqExt.infseq.
+Require Import StructTact.StructTactics.
+
+Section Shed.
+  (* The global state type. *)
+  Variable net : Type.
+  (* Relation defining whether one state can transition to another. *)
+  Variable step : net -> net -> Prop.
+  (* If steps are lengths of fence, operations are fenceposts. *)
+  Variable operation : Type.
+  (* You can "run" an operation on a net gst to produce another net
+     gst', provided the operation is valid to apply on that net, i.e.,
+     step gst gst' holds.
+
+     For example, an operation that crashes a node h won't be valid if
+     h isn't a live node. *)
+  Variable run : net -> operation -> option net.
+  (*
+  Variable run_valid :
+    forall gst op gst',
+      run gst op = Some gst' ->
+      step gst gst'.
+  Variable run_complete :
+    forall gst gst',
+      step gst gst' ->
+      exists op,
+        run gst op = Some gst'.*)
+
+  Definition run_lifted (gst : option net) (o : operation) : option net :=
+    match gst with
+    | Some gst' => run gst' o
+    | None => None
+    end.
+
+  (* Runs a list of operations starting at init. Only returns None if
+     one of the operations is invalid. *)
+  Definition run_all (ops : list operation) (init : net) : option net :=
+    fold_left run_lifted ops (Some init).
+
+  Definition valid_operation (gst : net) (op : operation) : Prop :=
+    exists gst',
+      run gst op = Some gst'.
+
+  (* A netpred is a decidable predicate on nets with a name. *)
+  Record netpred := { np_prop : net -> Prop;
+                      np_dec : forall gst, {np_prop gst} + {~ np_prop gst};
+                      np_name : string }.
+
+
+  Definition const_true {A} (_ : A) : Prop :=
+    True.
+
+  (* a sample netpred *)
+  Definition const_true_net_dec :
+    forall (gst : net),
+      {const_true gst} + {~ const_true gst}.
+  Proof.
+    intro gst.
+    now left.
+  Qed.
+
+  Definition np_const_true := {| np_prop := const_true;
+                                 np_dec := const_true_net_dec;
+                                 np_name := "np_const_true" |}.
+
+  (* Trace predicates are properties of infinite sequences, so we
+     can't actually test them. Instead we define a sort of decidable
+     version of a trace predicate that maps a finite list of
+     occurrences into the tp_result type. *)
+  Inductive tp_result : Set :=
+  | tp_True   (* I know for sure that it's true *)
+  | tp_False  (* I know for sure that it's false *)
+  | tp_Maybe. (* I need more information. *)
+
+  Definition tp_result_eq_dec :
+    forall (p q : tp_result),
+      {p = q} + {p <> q}.
+  Proof.
+    decide equality.
+  Defined.
+
+  (* prefix l s holds when s starts with the elements of l. *)
+  Inductive prefix {A} : list A -> infseq A -> Prop :=
+  | prefix_nil : forall s,
+      prefix [] s
+  | prefix_cons : forall x l s,
+      prefix l s ->
+      prefix (x :: l) (Cons x s).
+
+  Record occurrence := { occ_net : net;
+                         occ_op : operation }.
+  Definition occ_step (o o' : occurrence) : Prop :=
+    run (occ_net o) (occ_op o) = Some (occ_net o').
+
+  Inductive execution_prefix : list occurrence -> Prop :=
+  | ep_nil : execution_prefix []
+  | ep_one : forall o,
+      valid_operation (occ_net o) (occ_op o) ->
+      execution_prefix [o]
+  | ep_cons : forall l o o',
+      execution_prefix (o' :: l) -> 
+      occ_step o o' ->
+      execution_prefix (o :: o' :: l).
+
+  CoInductive execution : infseq occurrence -> Prop := 
+    exec_Cons : forall o o' s,
+      occ_step o o' ->
+      execution (Cons o' s) ->
+      execution (Cons o (Cons o' s)).
+
+  Definition tp_True_correct (tp_prop : infseq occurrence -> Prop) (tp_dec : list occurrence -> tp_result) (l : list occurrence) : Prop :=
+    tp_dec l = tp_True ->
+    forall s,
+      execution s ->
+      prefix l s ->
+      tp_prop s.
+
+  Definition tp_False_correct (tp_prop : infseq occurrence -> Prop) (tp_dec : list occurrence -> tp_result) (l : list occurrence) : Prop :=
+    tp_dec l = tp_False ->
+    forall s,
+      execution s ->
+      prefix l s ->
+      ~ tp_prop s.
+
+  Definition tp_Maybe_correct (tp_prop : infseq occurrence -> Prop) (tp_dec : list occurrence -> tp_result) (l : list occurrence) : Prop :=
+    tp_dec l = tp_Maybe ->
+    exists s s',
+      execution s /\ prefix l s /\ tp_prop s /\
+      execution s' /\ prefix l s /\ ~ tp_prop s'.
+
+  (* What it means for a tp_dec to do something *)
+  Definition tracepred_correct (tp_prop : infseq occurrence -> Prop) (tp_dec : list occurrence -> tp_result) : Prop :=
+    forall l,
+      tp_True_correct tp_prop tp_dec l \/
+      tp_False_correct tp_prop tp_dec l \/
+      tp_Maybe_correct tp_prop tp_dec l.
+
+  (* A tracepred is a predicate on infinite executions with a
+     decidable analogue defined on finite executions and a name. *)
+  Record tracepred := { tp_prop : infseq occurrence -> Prop;
+                        tp_dec : list occurrence -> tp_result;
+                        tp_correct : tracepred_correct tp_prop tp_dec;
+                        tp_name : string }.
+
+  Definition const_true_tp_dec (t : list occurrence) : tp_result :=
+    tp_True.
+
+  Definition const_true_tp_dec_correct :
+    tracepred_correct const_true const_true_tp_dec.
+  Proof.
+    left.
+    easy.
+  Defined.
+
+  Definition tp_const_true := {| tp_prop := const_true;
+                                 tp_dec := const_true_tp_dec;
+                                 tp_correct := const_true_tp_dec_correct;
+                                 tp_name := "tp_const_true" |}.
+
+  Definition is_tp_false (p : tp_result) : bool :=
+    if tp_result_eq_dec p tp_False
+    then true
+    else false.
+  
+  Definition any_tracepreds_false (preds : list tracepred) (l : list occurrence) : bool :=
+    existsb is_tp_false (map (fun p => tp_dec p l) preds).
+
+  Definition any_netpreds_false (preds : list netpred) (gst : net) : bool :=
+    existsb (Bool.eqb false) (map (fun p => proj_sumbool (np_dec p gst)) preds).
+
+  Record test_state := { (* trace of program thus far *)
+                         ts_trace : list occurrence; 
+                         (* latest state, since occurrences have a sort of fencepost issue *)
+                         ts_latest : net;
+                         ts_netpreds : list (netpred * list bool); 
+                         ts_tracepreds : list (tracepred * list tp_result);
+                         ts_error : option string }.
+
+  Definition extend_by (st : test_state) (gst : net) (op : operation) : test_state :=
+    {| ts_trace := ts_trace st ++ [{| occ_net := ts_latest st;
+                                      occ_op := op |}];
+       ts_latest := gst;
+       ts_netpreds := ts_netpreds st;
+       ts_tracepreds := ts_tracepreds st;
+       ts_error := ts_error st |}.
+
+  Definition try_step_test (st : test_state) (op : operation) : option test_state :=
+    match run (ts_latest st) op with
+    | Some gst' => Some (extend_by st gst' op)
+    | None => None
+    end.
+
+  Definition update_netpred_result (st : test_state) (npres : netpred * list bool) : netpred * list bool :=
+    let (np, results) := npres in
+    (np, (proj_sumbool (np_dec np (ts_latest st))) :: results).
+
+  Definition update_netpreds_results (st : test_state) : list (netpred * list bool) :=
+    map (update_netpred_result st) (ts_netpreds st).
+
+  Definition update_tracepred_result (st : test_state) (tpres : tracepred * list tp_result) : tracepred * list tp_result :=
+    let (tp, results) := tpres in
+    (tp, (tp_dec tp (ts_trace st)) :: results).
+
+  Definition update_tracepreds_results (st : test_state) : list (tracepred * list tp_result) :=
+    map (update_tracepred_result st) (ts_tracepreds st).
+
+  Definition add_checks_for_latest (st : test_state) : test_state :=
+    {| ts_trace := ts_trace st;
+       ts_latest := ts_latest st;
+       ts_netpreds := update_netpreds_results st;
+       ts_tracepreds := update_tracepreds_results st;
+       ts_error := ts_error st |}.
+
+  Definition set_error (st : test_state) s :=
+    {| ts_trace := ts_trace st;
+       ts_latest := ts_latest st;
+       ts_netpreds := ts_netpreds st;
+       ts_tracepreds := ts_tracepreds st;
+       ts_error := Some s |}.
+
+  Fixpoint random_test_body (st : test_state) (next : net -> nat -> operation) (n : nat) : test_state :=
+    let st_checked := add_checks_for_latest st in
+    match n with
+    | O => st
+    | S n' =>
+      match try_step_test st_checked (next (ts_latest st_checked) n) with
+      | Some st' => random_test_body st' next n'
+      | None => set_error st "planned an invalid operation"
+      end
+    end.
+
+  Definition pair_to_nil {A B: Type} (x : A) : A * (list B) :=
+    (x, []).
+
+  Definition make_initial_state (init : net) (netpreds : list netpred) (tracepreds : list tracepred) : test_state :=
+    {| ts_trace := [];
+       ts_latest := init;
+       ts_netpreds := map pair_to_nil netpreds;
+       ts_tracepreds := map pair_to_nil tracepreds;
+       ts_error := None |}.
+
+  Definition random_test (netpreds : list netpred) (tracepreds : list tracepred) (init : net) (next : net -> nat -> operation) (n : nat) : test_state :=
+    random_test_body (make_initial_state init netpreds tracepreds) next n.
+End Shed.
+
+Extraction "extraction/lib/ExtractedShed.ml" random_test np_const_true tp_const_true netpred.
